theories/iris_extra/persistence.v
@@ -13,7 +13,7 @@ Class CmraPersistent (M : cmraT) :=
 Section CmraPersistentLaws.
   Local Arguments uPred_holds {_} !_ _ _.
 
-  Global Instance CmraPersistent_Persistent {M : ucmraT} `(!CmraPersistent M)
+  #[global] Instance CmraPersistent_Persistent {M : ucmraT} `(!CmraPersistent M)
     (P : uPred M) : Persistent P.
   Proof.
     split => n x Hx Hpx; uPred.unseal.
